---
Crafted by [Genie](https://marketplace.visualstudio.com/items?itemName=genieai.chatgpt-vscode)

---

## You

Convert the following CFG into CNF
S → ASA | aB
A → B | S
B → b | ε

## Genie

To convert a CFG to CNF we have to follow these steps:

1. Eliminate ε-productions
2. Eliminate unit productions
3. Convert all productions to have only two variables or one terminal on the right-hand side

**Step 1: Eliminating ε-Productions**

The ε-production is `B → ε`, so we can remove it by adding new rules. Using `B → ε` implies that `S → ASε | a`. So, `S → ASA | SA | a`.

```
S → ASA | SA | a
A → B | S
B → b
```

**Step 2: Eliminating Unit Productions**

There are no unit productions in the current grammar.

**Step 3: Convert productions to CNF**

We have to make sure that each production has either:

- A single terminal symbol
- Two non-terminal symbols

Also, we need to add new variables if necessary.

Since our starting variable S has three symbols on the right-hand side, we need to introduce a new variable to make it work. We add a new variable X and replace S → ASA with the following two new rules:

- S → AX
- A → SA | aB
- X → SA

So, our final CNF grammar is:

```
S  → AX | a
A  → SA | aB
B  → b
X  → SA
```

## You

Convert the following grammar G into Greibach Normal Form (GNF).
A → aBD | bDB | c
A →AB | AD

## Genie

First, we need to eliminate left-recursion by creating a new non-terminal for each production.

```
A → aBD | bDB | c
A → AB | AD

Let's add A1 and A2 variables:

A  → aBDA1 | bDBA1 | cA2
A1 → BDA1 | DBA1
A2 → BA | DA
B  → b
D  → d
```

Now we need to convert the grammar to Greibach Normal Form. In GNF, all productions start with a terminal or epsilon. We can achieve this by replacing the non-terminals with their right-most derivations.

```
A   → aBD A1 | bDB A1 | cA2
A1  → bDA1 | dBA1 | ε
A2  → AB | AD
B   → b
D   → d
```

Now our grammar is in Greibach Normal Form.

## You

Construct PDA accepting the language
L= {an
b2n |n>0}

## Genie

We can construct the PDA for the language L = {anb2n | n > 0} as follows:

1. The PDA's stack alphabet is {Z}, where Z is the initial stack symbol.
2. The PDA's input alphabet is {a, b}.
3. The PDA's set of states is {q0, q1, q2, q3, q4}:
   - q0 is the start state
   - q1 is used to read input a and push it onto the stack
   - q2 is used to read input b and push two bs onto the stack
   - q3 is the accept state that is reached when all input has been consumed and the stack has only the initial Z on it
   - q4 is a dead state that is entered if the input doesn't match any possible string in the language
4. The transition function δ for the PDA is defined as follows:
   - δ(q0, a, Z) = (q1, Z)
   - δ(q1, a, Z) = (q1, aZ)
   - δ(q1, b, a) = (q2, aa)
   - δ(q2, b, a) = (q2, aaa)
   - δ(q2, ε, Z) = (q3, Z)
   - δ(q0, b, Z) = (q4, Z)  // entering a dead state

In words, the PDA operates as follows:

1. It reads an `a` from the input and pushes it onto the stack until there are n `a`s on the stack.
2. It reads a `b` from the input and pushes two `b`s onto the stack until there are 2n `b`s on the stack.
3. If all the input has been consumed and the stack contains only the initial symbol Z, it enters an accept state.
4. If it reads a `b` before reading an `a`, or if it reads an extra `a` after reading all the input, it enters a dead state.

This PDA recognizes the language L = {anb2n | n > 0}.

## You

Design a Non-Deterministic PDA for accepting the language L = {ww r ,w ∈ (a, b)*}

## Genie

We can design the NPDA for L = {wwr: w ∈ (a, b)* } as follows:

1. The PDA's stack alphabet is {Z}, where Z is the initial stack symbol.
2. The PDA's input alphabet is {a, b}.
3. The PDA's set of states is {q0, q1, q2, q3}:
   - q0 is the start state
   - q1 is used to read input `a` or `b` and push it onto the stack
   - q2 is used to compare the top of the stack with the input reading head and pop the stack if they are equal
   - q3 is the accept state that is reached when all input has been consumed and the stack is empty
4. The transition function δ for the PDA is defined as follows:
   - δ(q0, ε, Z) = {(q1, Z)}  // move to state q1 and start reading input
   - δ(q1, a, Z) = {(q1, aZ)}  // push input a onto stack
   - δ(q1, b, Z) = {(q1, bZ)}  // push input b onto stack
   - δ(q1, ε, Z) = {(q2, Z)}  // move to state q2 and start comparing input and stack contents
   - δ(q2, a, a) = {(q2, ε)}  // compare top of stack with input; if equal then pop both
   - δ(q2, b, b) = {(q2, ε)}  // compare top of stack with input; if equal then pop both
   - δ(q2, ε, Z) = {(q3, Z)}  // if we reach end of input and stack is empty, move to accept state

In words, the PDA operates as follows:

1. The PDA starts in the start state q0 and pushes a new Z onto the stack.
2. In state q1, it reads an input `a` or `b` and pushes it onto the stack until there is a complete copy of the input string on the stack.
3. In state q2, it compares the top of the stack with the input reading head and pops the stack if they are equal. It repeats this step until the stack is empty and the entire input has been consumed.
4. If all the input has been consumed and the stack is empty, it enters an accept state q3.

This NPDA recognizes the language L = {wwr: w ∈ (a, b)*}.

## You

State closure properties of Context Free Language with examples.

## Genie

The closure properties of context-free languages refer to the properties that are preserved when we perform certain operations on a language. These properties are useful for proving various theorems about context-free languages and for developing algorithms that manipulate or transform them.

Here are some closure properties of context-free languages along with examples:

1. **Union:** The union of two context-free languages is also a context-free language.
   - Example: Let L1 = {a^n b^n | n ≥ 0} and L2 = {a^n b^m | n, m ≥ 0}. Then, L1 ∪ L2 = {a^n b^m | n, m ≥ 0} is also a context-free language.

2. **Concatenation:** The concatenation of two context-free languages is also a context-free language.
   - Example: Let L1 = {a^n b^n | n ≥ 0} and L2 = {c^m d^m | m ≥ 0}. Then, L1L2 = {a^n b^n c^m d^m | n, m ≥ 0} is also a context-free language.

3. **Intersection:** The intersection of a context-free language and a regular language is a context-free language.
   - Example: Let L1 = {a^n b^n | n ≥ 0} and L2 = {a^* b^* c^*}. Then, L1 ∩ L2 = {a^n b^n c^m | n, m ≥ 0} is also a context-free language.

4. **Complement:** The complement of a context-free language is not necessarily a context-free language.
   - Example: Let L = {a^n b^n | n ≥ 0}. Then, the complement of L is {w | w ∈ (a ∪ b)^* and w ∉ L} which is not context-free.

5. **Kleene Star:** The Kleene star of a context-free language is also a context-free language.
   - Example: Let L = {a^n b^n | n ≥ 0}. Then, L* = {ε, ab, aabb, aaabbb, ...} is also a context-free language.

6. **Homomorphism:** If h is a homomorphism from Σ* to Γ*, then h(L) is a context-free language for any context-free language L over Σ.
   - Example: Let h be the homomorphism defined by h(a) = x and h(b) = y. Let L = {a^n b^m | n, m ≥ 0}. Then, h(L) = {x^n y^m | n, m ≥ 0} is also a context-free language.

7. **Inverse Homomorphism:** If h is a homomorphism from Σ* to Γ*, and L is a context-free language over Γ, then h^{-1}(L) is a context-free language over Σ.
   - Example: Let h be the homomorphism defined by h(a) = x and h(b) = y. Let L = {x^n y^m | n, m ≥ 0}. Then, h^{-1}(L) = {a^n b^m | n, m ≥ 0} is also a context-free language.